src/InvariantProofs.v
@@ -18,9 +18,46 @@
   along with this program; if not, write to the Free Software
   Foundation, Inc., 51 Franklin St, Fifth Floor, Boston, MA  02110-1301 USA *)
 
-Require Import Rcore Rfeatures Rinit.
+Require Import Rcore RfeaturesAux Rinit.
 Require Export Invariants.
 
+(** * General Lemmae **)
+
+(** If runs returns a result, then adding fuel does not change it. **)
+Lemma runs_while_loop_fuel_conserve : forall A globals n n' S (a : A) expr body,
+    n <= n' ->
+    ~ bottom_result (runs_while_loop (runs n globals) S a expr body) ->
+    runs_while_loop (runs n' globals) S a expr body = runs_while_loop (runs n globals) S a expr body.
+Proof.
+  introv I B. repeat rewrite <- runs_proj_while_loop_eq in *. gen n' S a. induction n; introv I B.
+  - false~ B.
+  - destruct n'; try solve [ math ]. simpls. unfolds while_loop. repeat rewrite <- runs_proj_while_loop_eq.
+    destruct expr; simpls~; tryfalse~. cases_if~.
+    destruct body; simpls~; tryfalse~. rewrite~ IHn. math.
+Qed.
+
+(* Slow version
+Lemma runs_while_loop_fuel_conserve : forall A globals n n' S (a : A) expr body,
+    n <= n' ->
+    ~ bottom_result (runs_while_loop (runs n globals) S a expr body) ->
+    runs_while_loop (runs n' globals) S a expr body = runs_while_loop (runs n globals) S a expr body.
+Proof.
+  introv I B. gen n' S a. induction n; introv I B.
+  - false~ B.
+  - destruct n'; try solve [ math ]. simpls. unfolds while_loop. repeat rewrite <- runs_proj_while_loop_eq.
+    destruct expr; simpls~; tryfalse~. cases_if~.
+    destruct body; simpls~; tryfalse~. rewrite~ IHn. math.
+Qed.
+*)
+
+(* TODO: put these lemmae in RfeaturesAux.v.
+   In RfeaturesAux, we can change the tactic to work on all projections
+   by only unfolding everything in aux1 (no simplifications), then do a
+   simplification between the two auxn.
+   We will then be able to automate the lemmae above, without them taking
+   too much time to compile. *)
+
+(** * Lemmae about Rinit.v **)
 
 (* TODO *)
 
@@ -29,6 +66,4 @@ Require Export Invariants.
 
 (** It would be nice to prove that the read-eval-print-loop can not
   return a [result_impossible]. **)
-
-(** If runs returns a result, then adding fuel does not change it. **)
 
