src/RfeaturesAux.v
@@ -1,0 +1,233 @@
+(** RfeaturesAux.
+  Contains useful lemmae about [runs]. **)
+
+(* Copyright © 2018 Martin Bodin
+
+  This program is free software; you can redistribute it and/or modify
+  it under the terms of the GNU General Public License as published by
+  the Free Software Foundation; either version 2 of the License, or
+  (at your option) any later version.
+
+  This program is distributed in the hope that it will be useful,
+  but WITHOUT ANY WARRANTY; without even the implied warranty of
+  MERCHANTABILITY or FITNESS FOR A PARTICULAR PURPOSE.  See the
+  GNU General Public License for more details.
+
+  You should have received a copy of the GNU General Public License
+  along with this program; if not, write to the Free Software
+  Foundation, Inc., 51 Franklin St, Fifth Floor, Boston, MA  02110-1301 USA *)
+
+Require Export Rfeatures.
+
+
+(** * Projections of [runs] **)
+
+(** As-is, [runs] is a large definition and [simpl] can take a while if
+  there is a [runs] to unfold in the context.  We would sometimes want
+  to only consider a simpler definition of [runs] containing only the
+  interesting projection. **)
+
+(** ** Tactics **)
+
+(** All these definitions follow a similar pattern.
+  We thus automate their definitions using tactics. **)
+
+(** Get the expected type of the replacement projection. **)
+Ltac get_type_projection proj :=
+  match type of proj with
+  | runs_type -> ?t => exact (nat -> Globals -> t)
+  end.
+
+(** Defines the projection for the cases where the function behind
+  the projection is a simple recursive loop. **)
+Ltac compute_simple_projection proj :=
+  let globals := fresh "globals" in
+  let max_step := fresh "max_step" in
+  let IHmax_step := fresh "IH" max_step in
+  intros max_step globals;
+  induction max_step as [|max_step IHmax_step];
+  [ let r := eval simpl in (proj (runs 0 globals)) in exact r
+  | let r := eval simpl in (proj (runs (S max_step) globals)) in
+    let rec aux1 r :=
+      match r with
+      | context [ ?f (runs max_step globals) ] =>
+        lazymatch f with
+        | proj => fail
+        | ?f' globals =>
+          let r := eval unfold f' in r in
+          let r := eval simpl in r in
+          aux1 r
+        | _ _ => fail
+        | _ =>
+          let r := eval unfold f in r in
+          let r := eval simpl in r in
+          aux1 r
+        end
+      | _ => r
+      end in
+    let r := aux1 r in
+    let rec aux2 r :=
+      match r with
+      | context C [ proj (runs max_step globals) ] =>
+        let r := context C[IHmax_step] in
+        aux2 r
+      | context C [ proj globals (runs max_step globals) ] =>
+        let r := context C[IHmax_step] in
+        aux2 r
+      | _ => r
+      end in
+    let r := aux2 r in
+    exact r ].
+
+(** Solves the equality when the function behind the projection
+  is a simple recursive loop. **)
+Ltac solve_eq_simple_projection :=
+  let globals := fresh "globals" in
+  let max_step := fresh "max_step" in
+  let IHmax_step := fresh "IH" max_step in
+  intros max_step globals; induction max_step as [|max_step IHmax_step];
+  [ reflexivity
+  | simpl; repeat rewrite <- IHmax_step; reflexivity ].
+
+(** ** [runs_while_loop] **)
+
+Definition runs_proj_while_loop : ltac:(get_type_projection runs_while_loop).
+  compute_simple_projection runs_while_loop.
+Defined.
+
+Lemma runs_proj_while_loop_eq : forall max_step globals,
+  runs_while_loop (runs max_step globals) = runs_proj_while_loop max_step globals.
+Proof. solve_eq_simple_projection. Qed.
+
+(** ** [runs_set_longjump] **)
+
+Definition runs_proj_set_longjump : ltac:(get_type_projection runs_set_longjump).
+  compute_simple_projection runs_set_longjump.
+Defined.
+
+Lemma runs_proj_set_longjump_eq : forall max_step globals,
+  runs_set_longjump (runs max_step globals) = runs_proj_set_longjump max_step globals.
+Proof. solve_eq_simple_projection. Qed.
+
+(** ** [runs_R_cycle_detected] **)
+
+Definition runs_proj_R_cycle_detected : ltac:(get_type_projection runs_R_cycle_detected).
+  compute_simple_projection runs_R_cycle_detected.
+Defined.
+
+Lemma runs_proj_R_cycle_detected_eq : forall max_step globals,
+  runs_R_cycle_detected (runs max_step globals) = runs_proj_R_cycle_detected max_step globals.
+Proof. solve_eq_simple_projection. Qed.
+
+(** ** [runs_eval] **)
+
+(** Unfortunately, this cases uses other functions, making it difficult to produce such a definition. **)
+
+(** ** [runs_getAttrib] **)
+
+(** Unfortunately, this cases uses other functions, making it difficult to produce such a definition. **)
+
+(** ** [runs_setAttrib] **)
+
+(** Unfortunately, this cases uses other functions, making it difficult to produce such a definition. **)
+
+(** ** [runs_duplicate1] **)
+
+(** Unfortunately, this cases uses other functions, making it difficult to produce such a definition. **)
+
+(** ** [runs_stripAttrib] **)
+
+Definition runs_proj_stripAttrib : ltac:(get_type_projection runs_stripAttrib).
+  compute_simple_projection runs_stripAttrib.
+Defined.
+
+Lemma runs_proj_stripAttrib_eq : forall max_step globals,
+  runs_stripAttrib (runs max_step globals) = runs_proj_stripAttrib max_step globals.
+Proof. solve_eq_simple_projection. Qed.
+
+(** ** [runs_evalseq] **)
+
+(** Unfortunately, this cases uses other functions, making it difficult to produce such a definition. **)
+
+(** ** [runs_R_isMissing] **)
+
+(** Unfortunately, this cases uses other functions, making it difficult to produce such a definition. **)
+
+(** ** [runs_AnswerType] **)
+
+(** Unfortunately, this cases uses other functions, making it difficult to produce such a definition. **)
+
+(** ** [runs_ListAnswer] **)
+
+Definition runs_proj_ListAnswer : ltac:(get_type_projection runs_ListAnswer).
+  compute_simple_projection runs_ListAnswer.
+Defined.
+
+Lemma runs_proj_ListAnswer_eq : forall max_step globals,
+  runs_ListAnswer (runs max_step globals) = runs_proj_ListAnswer max_step globals.
+Proof. solve_eq_simple_projection. Qed.
+
+(** ** [runs_StringAnswer] **)
+
+(** Unfortunately, this cases uses other functions, making it difficult to produce such a definition. **)
+
+(** ** [runs_LogicalAnswer] **)
+
+Definition runs_proj_LogicalAnswer : ltac:(get_type_projection runs_LogicalAnswer).
+  compute_simple_projection runs_LogicalAnswer.
+Defined.
+
+Lemma runs_proj_LogicalAnswer_eq : forall max_step globals,
+  runs_LogicalAnswer (runs max_step globals) = runs_proj_LogicalAnswer max_step globals.
+Proof. solve_eq_simple_projection. Qed.
+
+(** ** [runs_IntegerAnswer] **)
+
+Definition runs_proj_IntegerAnswer : ltac:(get_type_projection runs_IntegerAnswer).
+  compute_simple_projection runs_IntegerAnswer.
+Defined.
+
+Lemma runs_proj_IntegerAnswer_eq : forall max_step globals,
+  runs_IntegerAnswer (runs max_step globals) = runs_proj_IntegerAnswer max_step globals.
+Proof. solve_eq_simple_projection. Qed.
+
+(** ** [runs_RealAnswer] **)
+
+Definition runs_proj_RealAnswer : ltac:(get_type_projection runs_RealAnswer).
+  compute_simple_projection runs_RealAnswer.
+Defined.
+
+Lemma runs_proj_RealAnswer_eq : forall max_step globals,
+  runs_RealAnswer (runs max_step globals) = runs_proj_RealAnswer max_step globals.
+Proof. solve_eq_simple_projection. Qed.
+
+(** ** [runs_ComplexAnswer] **)
+
+Definition runs_proj_ComplexAnswer : ltac:(get_type_projection runs_ComplexAnswer).
+  compute_simple_projection runs_ComplexAnswer.
+Defined.
+
+Lemma runs_proj_ComplexAnswer_eq : forall max_step globals,
+  runs_ComplexAnswer (runs max_step globals) = runs_proj_ComplexAnswer max_step globals.
+Proof. solve_eq_simple_projection. Qed.
+
+(** ** [runs_RawAnswer] **)
+
+Definition runs_proj_RawAnswer : ltac:(get_type_projection runs_RawAnswer).
+  compute_simple_projection runs_RawAnswer.
+Defined.
+
+Lemma runs_proj_RawAnswer_eq : forall max_step globals,
+  runs_RawAnswer (runs max_step globals) = runs_proj_RawAnswer max_step globals.
+Proof. solve_eq_simple_projection. Qed.
+
+(** ** [runs_R_FunTab] **)
+
+Definition runs_proj_R_FunTab : ltac:(get_type_projection runs_R_FunTab).
+  compute_simple_projection runs_R_FunTab.
+Defined.
+
+Lemma runs_proj_R_FunTab_eq : forall max_step globals,
+  runs_R_FunTab (runs max_step globals) = runs_proj_R_FunTab max_step globals.
+Proof. solve_eq_simple_projection. Qed.
+
